added cont, tspf_well prove for medRS
the medRS proves can be used to instantiate the mdia as TSPS,
concerns #136

CaseStudies/ABP/ABP_TSPS.thy
@@ -7,20 +7,20 @@
 
 theory ABP_TSPS
   imports "../../TSPS" Receiver Composition Medium "../../TSPF"
-    
+
 begin
 
   default_sort countable
-  
+
 (* ----------------------------------------------------------------------- *)
 section \<open>Datatype Definition\<close>
 (* ----------------------------------------------------------------------- *)
-  
+
 datatype 'a::countable MABP = BoolPair "('a * bool)" | Bool bool | Data 'a
 
 instantiation MABP ::  (countable) countable
 begin
-instance 
+instance
    by (countable_datatype)
 end
 
@@ -41,11 +41,11 @@ end
  declare [[show_types]]
   declare [[show_sorts]]
 declare [[show_consts]]
-  
+
 (* ----------------------------------------------------------------------- *)
 section \<open>Definitions\<close>
-(* ----------------------------------------------------------------------- *)  
- 
+(* ----------------------------------------------------------------------- *)
+
 subsection \<open>datatype destructors\<close>
 abbreviation invBoolPair :: "'a MABP \<Rightarrow> ('a \<times> bool)" where
 "invBoolPair \<equiv> (inv BoolPair)"
@@ -57,13 +57,13 @@ abbreviation invData :: "'a MABP \<Rightarrow> 'a" where
 "invData \<equiv> (inv Data)"
 
 abbreviation recvAbb where
-"recvAbb \<equiv> 
+"recvAbb \<equiv>
 let recRes = (\<lambda> x. tsRec\<cdot>((tsMap invBoolPair)\<cdot>(x . dr)))
 in (\<lambda> x. (tsbDom\<cdot>x = {dr}) \<leadsto> [ar    \<mapsto> tsMap Bool\<cdot>(fst (recRes x)),
-                                        abpOut \<mapsto> tsMap Data\<cdot>(snd (recRes x))]\<Omega>)" 
-  
+                                        abpOut \<mapsto> tsMap Data\<cdot>(snd (recRes x))]\<Omega>)"
 
-subsection \<open>receiver\<close> 
+
+subsection \<open>receiver\<close>
 definition recvTSPF :: "'a MABP TSPF" where
 "recvTSPF \<equiv> Abs_CTSPF (\<lambda> x. (tsbDom\<cdot>x = {dr}) \<leadsto> [ar    \<mapsto> (tsMap::(bool \<Rightarrow> 'a MABP) \<Rightarrow> bool tstream \<rightarrow> 'a MABP tstream) Bool\<cdot>(fst ( tsRec\<cdot>((tsMap invBoolPair)\<cdot>(x . dr)))),
                                         abpOut \<mapsto> (tsMap::('a \<Rightarrow> 'a MABP) \<Rightarrow> 'a tstream \<rightarrow> 'a MABP tstream) Data\<cdot>(snd ( tsRec\<cdot>((tsMap invBoolPair)\<cdot>(x . dr))))]\<Omega>)"
@@ -71,113 +71,119 @@ definition recvTSPF :: "'a MABP TSPF" where
 subsection \<open>medium_rs\<close>
   (* medium from receiver to sender *)
   (* input: ar, output: as, transport booleans *)
-  
+
 definition tsMedRSTSPF :: "bool stream \<Rightarrow> 'a MABP TSPF" where
-"tsMedRSTSPF bst\<equiv> Abs_CTSPF (\<lambda> x. (tsbDom\<cdot>x = {ar}) 
-                                    \<leadsto> [as \<mapsto> tsMap Bool\<cdot>(tsMed\<cdot>(tsMap invBool\<cdot>(x . ar))\<cdot>bst)]\<Omega>)"
-  
+"tsMedRSTSPF bst\<equiv> Abs_CTSPF (\<lambda> x. (tsbDom\<cdot>x = {ar})
+                           \<leadsto> [as \<mapsto> (tsMap::(bool \<Rightarrow> 'a MABP) \<Rightarrow> bool tstream \<rightarrow> 'a MABP tstream) Bool\<cdot>(tsMed\<cdot>(tsMap invBool\<cdot>(x . ar))\<cdot>bst)]\<Omega>)"
+
+abbreviation tsMedRSAbb  :: "bool stream \<Rightarrow> 'a MABP TSB \<Rightarrow> 'a MABP TSB option" where
+"tsMedRSAbb bst x \<equiv> ((tsbDom\<cdot>x = {ar})
+                           \<leadsto> [as \<mapsto> (tsMap::(bool \<Rightarrow> 'a MABP) \<Rightarrow> bool tstream \<rightarrow> 'a MABP tstream) Bool\<cdot>(tsMed\<cdot>(tsMap invBool\<cdot>(x . ar))\<cdot>bst)]\<Omega>)"
+
 subsection \<open>medium_sr\<close>
   (* medium from sender to receiver *)
   (* input: ds, output: dr, transport (data, bool) tuples *)
-  
+
+
+  (* TODO: fix types *)
 definition tsMedSRTSPF :: "bool stream \<Rightarrow> 'a MABP TSPF" where
-"tsMedSRTSPF bst\<equiv> Abs_CTSPF (\<lambda> x. (tsbDom\<cdot>x = {ds}) 
+"tsMedSRTSPF bst\<equiv> Abs_CTSPF (\<lambda> x. (tsbDom\<cdot>x = {ds})
                                 \<leadsto> [dr \<mapsto> tsMap BoolPair\<cdot>(tsMed\<cdot>(tsMap invBoolPair\<cdot>(x . ds))\<cdot>bst)]\<Omega>)"
 
 
 (* ----------------------------------------------------------------------- *)
 section \<open>lemmata\<close>
-(* ----------------------------------------------------------------------- *) 
-  
+(* ----------------------------------------------------------------------- *)
+
 subsection \<open>general\<close>
-  
+
 lemma tsmap_id[simp]: assumes "inj f" shows "tsMap (inv f)\<cdot>(tsMap f\<cdot>ts) = ts"
 apply(induction ts)
 by(simp_all add: assms tsmap_delayfun  tsmap_mlscons)
- 
-subsection \<open>datatype\<close>  
-  
+
+subsection \<open>datatype\<close>
+
   (* inverse BoolPair applied to BoolPair is identity *)
 lemma data_bool_pair_inv [simp]: "(invBoolPair) (BoolPair x) = x"
   by (meson MABP.inject(1) f_inv_into_f rangeI)
-  
+
   (* inverse Bool applied to Bool is identity *)
 lemma data_bool_inv [simp]: "(inv Bool) (Bool x) = x"
   by (meson MABP.inject(2) f_inv_into_f rangeI)
-    
+
   (* inverse Data applied to Data is identity *)
 lemma data_data_inv [simp]: "(inv Data) (Data x) = x"
   by (meson MABP.inject(3) f_inv_into_f rangeI)
-  
+
 
 subsection \<open>receiver\<close>
 
-subsubsection \<open>defs\<close>  
-  
+subsubsection \<open>defs\<close>
+
       (* helper functions to prove cont *)
 definition recvCH1 :: "'a MABP TSB \<Rightarrow> 'a MABP tstream"  where
 "recvCH1 \<equiv> (\<lambda> x. tsMap Bool\<cdot>(fst (tsRec\<cdot>((tsMap invBoolPair)\<cdot>(x .dr)))))"
-    
+
 definition recvCH2 :: "'a MABP TSB \<Rightarrow> 'a MABP tstream"  where
 "recvCH2 \<equiv> (\<lambda> x. tsMap Data\<cdot>(snd (tsRec\<cdot>((tsMap invBoolPair)\<cdot>(x .dr)))))"
-  
-lemma recvCH1_contlub: assumes "  chain Y" and "tsbDom\<cdot>(\<Squnion>i::nat. Y i) = {dr}"
+
+lemma recvCH1_contlub: assumes "chain Y"
   shows "recvCH1 ((\<Squnion>i. Y i)) = (\<Squnion>i. (recvCH1 ((Y i))))"
   apply (rule cont2contlubE)
   by (simp_all add: assms recvCH1_def)
-    
-lemma recvCH2_contlub: assumes "  chain Y" and "tsbDom\<cdot>(\<Squnion>i::nat. Y i) = {dr}"
+
+lemma recvCH2_contlub: assumes "chain Y"
   shows "recvCH2 ((\<Squnion>i. Y i)) = (\<Squnion>i. (recvCH2 ((Y i))))"
   apply (rule cont2contlubE)
   by (simp_all add: assms recvCH2_def)
 
-    
-lemma to_recvch1: "tsMap Bool\<cdot>(fst (tsRec\<cdot>((tsMap invBoolPair)\<cdot>(x .dr)))) 
+
+lemma to_recvch1: "tsMap Bool\<cdot>(fst (tsRec\<cdot>((tsMap invBoolPair)\<cdot>(x .dr))))
                     = (recvCH1::'a MABP TSB \<Rightarrow> 'a MABP tstream) x"
   by (simp add: recvCH1_def)
-    
-lemma to_recvch2: "tsMap Data\<cdot>(snd (tsRec\<cdot>((tsMap invBoolPair)\<cdot>(x .dr)))) 
+
+lemma to_recvch2: "tsMap Data\<cdot>(snd (tsRec\<cdot>((tsMap invBoolPair)\<cdot>(x .dr))))
                     = (recvCH2::'a MABP TSB \<Rightarrow> 'a MABP tstream) x"
   by (simp add: recvCH2_def)
-  
-   
- 
-    
-    
+
+
+
+
+
 lemma recv_tsb_well [simp]:
   shows "tsb_well [ar \<mapsto> tsMap Bool\<cdot>(fst (tsRec\<cdot>((tsMap invBoolPair)\<cdot>(x . dr)))),
                                   abpOut \<mapsto> tsMap Data\<cdot>(snd (tsRec\<cdot>((tsMap invBoolPair)\<cdot>(x . dr))))]"
   apply (rule tsb_wellI)
   apply (simp add: tsmap_tsdom_range)
   by blast
-    
+
 lemma recv_tsb_dom: "tsbDom\<cdot>([ar \<mapsto> tsMap Bool\<cdot>(fst (tsRec\<cdot>((tsMap invBoolPair)\<cdot>(x . dr)))),
-                              abpOut \<mapsto> tsMap Data\<cdot>(snd (tsRec\<cdot>((tsMap invBoolPair)\<cdot>(x . dr))))]\<Omega>) 
+                              abpOut \<mapsto> tsMap Data\<cdot>(snd (tsRec\<cdot>((tsMap invBoolPair)\<cdot>(x . dr))))]\<Omega>)
                      = {ar, abpOut}"
   apply (simp add: tsbdom_rep_eq)
     by auto
 
-subsubsection \<open>cont\<close>       
-      
-lemma rec_tsb_mono: "\<And>(x::'a MABP TSB) y::'a MABP TSB. tsbDom\<cdot>x = {dr} \<Longrightarrow> x \<sqsubseteq> y \<Longrightarrow> 
-          [ar \<mapsto> tsMap Bool\<cdot>(fst (tsRec\<cdot>(tsMap invBoolPair\<cdot>(x  .  dr)))), 
-          abpOut \<mapsto> tsMap Data\<cdot>(snd (tsRec\<cdot>(tsMap invBoolPair\<cdot>(x  .  dr))))]\<Omega> 
-          \<sqsubseteq> [ar \<mapsto> tsMap Bool\<cdot>(fst (tsRec\<cdot>(tsMap invBoolPair\<cdot>(y  .  dr)))), 
+
+
+lemma rec_tsb_mono: "\<And>(x::'a MABP TSB) y::'a MABP TSB. tsbDom\<cdot>x = {dr} \<Longrightarrow> x \<sqsubseteq> y \<Longrightarrow>
+          [ar \<mapsto> tsMap Bool\<cdot>(fst (tsRec\<cdot>(tsMap invBoolPair\<cdot>(x  .  dr)))),
+          abpOut \<mapsto> tsMap Data\<cdot>(snd (tsRec\<cdot>(tsMap invBoolPair\<cdot>(x  .  dr))))]\<Omega>
+          \<sqsubseteq> [ar \<mapsto> tsMap Bool\<cdot>(fst (tsRec\<cdot>(tsMap invBoolPair\<cdot>(y  .  dr)))),
              abpOut \<mapsto> tsMap Data\<cdot>(snd (tsRec\<cdot>(tsMap invBoolPair\<cdot>(y  .  dr))))]\<Omega>"
       apply (rule tsb_below)
        apply (simp_all add: tsbdom_below tsbdom_rep_eq tsbgetch_rep_eq)
        by (simp add: fst_monofun snd_monofun monofun_cfun_arg tsbgetch_below)
-     
-  
-lemma recvTSPF_mono [simp]: "monofun (\<lambda> x. (tsbDom\<cdot>x = {dr}) \<leadsto> 
+
+
+lemma recvTSPF_mono [simp]: "monofun (\<lambda> x. (tsbDom\<cdot>x = {dr}) \<leadsto>
                                     [ar \<mapsto> tsMap Bool\<cdot>(fst (tsRec\<cdot>((tsMap invBoolPair)\<cdot>(x . dr)))),
                                      abpOut \<mapsto> tsMap Data\<cdot>(snd (tsRec\<cdot>((tsMap invBoolPair)\<cdot>(x . dr))))]\<Omega>)"
   apply (rule tspf_monoI)
   apply (rule tsb_below)
    apply (simp_all add: tsbdom_below tsbdom_rep_eq tsbgetch_rep_eq)
    by (simp add: fst_monofun snd_monofun monofun_cfun_arg tsbgetch_below)
-  
-     
+
+
 lemma recvTSPF_tsb_getc: assumes "chain Y" and "tsbDom\<cdot>(\<Squnion>i. Y i) = {dr}"
   and "c \<in>  {ar, abpOut}"
   shows " (\<Squnion>i.
@@ -188,77 +194,77 @@ lemma recvTSPF_tsb_getc: assumes "chain Y" and "tsbDom\<cdot>(\<Squnion>i. Y i) 
 proof (rule lubgetCh)
    have f2: "\<And> i. tsbDom\<cdot>(Y i) =  tsbDom\<cdot>(\<Squnion>i. Y i)"
      by (simp add: assms(1))
-   show tb_chain: "chain (\<lambda>i::nat. [ar \<mapsto> tsMap Bool\<cdot>(fst (tsRec\<cdot>(tsMap invBoolPair\<cdot>(Y i  .  dr)))), 
+   show tb_chain: "chain (\<lambda>i::nat. [ar \<mapsto> tsMap Bool\<cdot>(fst (tsRec\<cdot>(tsMap invBoolPair\<cdot>(Y i  .  dr)))),
                              abpOut \<mapsto> tsMap Data\<cdot>(snd (tsRec\<cdot>(tsMap invBoolPair\<cdot>(Y i  .  dr))))]\<Omega>)"
      by (simp add: assms(1) assms(2) po_class.chainE po_class.chainI rec_tsb_mono)
-   
-   show " c \<in> tsbDom\<cdot>(\<Squnion>i::nat. 
-                          [ar \<mapsto> tsMap Bool\<cdot>(fst (tsRec\<cdot>(tsMap invBoolPair\<cdot>(Y i  .  dr)))), 
+
+   show " c \<in> tsbDom\<cdot>(\<Squnion>i::nat.
+                          [ar \<mapsto> tsMap Bool\<cdot>(fst (tsRec\<cdot>(tsMap invBoolPair\<cdot>(Y i  .  dr)))),
                        abpOut \<mapsto> tsMap Data\<cdot>(snd (tsRec\<cdot>(tsMap invBoolPair\<cdot>(Y i  .  dr))))]\<Omega>)"
      using assms(3) recv_tsb_dom tb_chain tsbChain_dom_eq2 by blast
 qed
-   
-     
+
+
 
   (* show that recTSPF is cont, proof concept taken from TSPF_Template_CaseStudy *)
-lemma recvTSPF_cont [simp]: 
-  shows "cont (\<lambda> x. (tsbDom\<cdot>x = {dr}) \<leadsto> 
-                      [ar \<mapsto> (tsMap::(bool \<Rightarrow> 'a MABP) \<Rightarrow> bool tstream \<rightarrow> 'a MABP tstream) 
+lemma recvTSPF_cont [simp]:
+  shows "cont (\<lambda> x. (tsbDom\<cdot>x = {dr}) \<leadsto>
+                      [ar \<mapsto> (tsMap::(bool \<Rightarrow> 'a MABP) \<Rightarrow> bool tstream \<rightarrow> 'a MABP tstream)
                             Bool\<cdot>(fst ((tsRec::('a * bool) tstream \<rightarrow> (bool tstream \<times> 'a tstream))\<cdot>
                             ((tsMap invBoolPair)\<cdot>(x . dr)))),
-                       abpOut \<mapsto> (tsMap::('a \<Rightarrow> 'a MABP) \<Rightarrow> 'a tstream \<rightarrow> 'a MABP tstream) 
+                       abpOut \<mapsto> (tsMap::('a \<Rightarrow> 'a MABP) \<Rightarrow> 'a tstream \<rightarrow> 'a MABP tstream)
                             Data\<cdot>(snd (tsRec\<cdot>((tsMap invBoolPair)\<cdot>(x . dr))))]\<Omega>)"
   proof (rule tspf_contI)
-    show recv_mono: "\<And>(x::'a MABP TSB) y::'a MABP TSB. tsbDom\<cdot>x = {dr} \<Longrightarrow> x \<sqsubseteq> y \<Longrightarrow> 
-          [ar \<mapsto> tsMap Bool\<cdot>(fst (tsRec\<cdot>(tsMap invBoolPair\<cdot>(x  .  dr)))), 
-          abpOut \<mapsto> tsMap Data\<cdot>(snd (tsRec\<cdot>(tsMap invBoolPair\<cdot>(x  .  dr))))]\<Omega> 
-          \<sqsubseteq> [ar \<mapsto> tsMap Bool\<cdot>(fst (tsRec\<cdot>(tsMap invBoolPair\<cdot>(y  .  dr)))), 
+    show recv_mono: "\<And>(x::'a MABP TSB) y::'a MABP TSB. tsbDom\<cdot>x = {dr} \<Longrightarrow> x \<sqsubseteq> y \<Longrightarrow>
+          [ar \<mapsto> tsMap Bool\<cdot>(fst (tsRec\<cdot>(tsMap invBoolPair\<cdot>(x  .  dr)))),
+          abpOut \<mapsto> tsMap Data\<cdot>(snd (tsRec\<cdot>(tsMap invBoolPair\<cdot>(x  .  dr))))]\<Omega>
+          \<sqsubseteq> [ar \<mapsto> tsMap Bool\<cdot>(fst (tsRec\<cdot>(tsMap invBoolPair\<cdot>(y  .  dr)))),
              abpOut \<mapsto> tsMap Data\<cdot>(snd (tsRec\<cdot>(tsMap invBoolPair\<cdot>(y  .  dr))))]\<Omega>"
       by (simp add: rec_tsb_mono)
-      
-    have f1: " \<And>Y::nat \<Rightarrow> 'a MABP TSB. chain Y \<Longrightarrow> tsbDom\<cdot>(\<Squnion>i::nat. Y i) = {dr} \<Longrightarrow> 
-                tsbDom\<cdot>(\<Squnion>i::nat. [ar \<mapsto> tsMap Bool\<cdot>(fst (tsRec\<cdot>(tsMap invBoolPair\<cdot>(Y i  .  dr)))), 
+
+    have f1: " \<And>Y::nat \<Rightarrow> 'a MABP TSB. chain Y \<Longrightarrow> tsbDom\<cdot>(\<Squnion>i::nat. Y i) = {dr} \<Longrightarrow>
+                tsbDom\<cdot>(\<Squnion>i::nat. [ar \<mapsto> tsMap Bool\<cdot>(fst (tsRec\<cdot>(tsMap invBoolPair\<cdot>(Y i  .  dr)))),
                 abpOut \<mapsto> tsMap Data\<cdot>(snd (tsRec\<cdot>(tsMap invBoolPair\<cdot>(Y i  .  dr))))]\<Omega>) = {abpOut, ar}"
      proof -
       fix Y :: "nat \<Rightarrow> 'a MABP TSB"
       assume a1: "chain Y"
       assume a2: "tsbDom\<cdot>(\<Squnion>i. Y i) = {dr}"
-      have f3: "\<forall>t ta. (tsbDom\<cdot>t \<noteq> {dr} \<or> t \<notsqsubseteq> ta) 
-                        \<or> [ar \<mapsto> tsMap Bool\<cdot> (fst (tsRec\<cdot>(tsMap invBoolPair\<cdot>(t . dr)))), 
-                            abpOut \<mapsto> tsMap Data\<cdot> (snd (tsRec\<cdot> (tsMap invBoolPair\<cdot> (t . dr)))::'a tstream)]\<Omega> 
-                          \<sqsubseteq> [ar \<mapsto> tsMap Bool\<cdot> (fst (tsRec\<cdot>(tsMap invBoolPair\<cdot>(ta . dr)))), 
+      have f3: "\<forall>t ta. (tsbDom\<cdot>t \<noteq> {dr} \<or> t \<notsqsubseteq> ta)
+                        \<or> [ar \<mapsto> tsMap Bool\<cdot> (fst (tsRec\<cdot>(tsMap invBoolPair\<cdot>(t . dr)))),
+                            abpOut \<mapsto> tsMap Data\<cdot> (snd (tsRec\<cdot> (tsMap invBoolPair\<cdot> (t . dr)))::'a tstream)]\<Omega>
+                          \<sqsubseteq> [ar \<mapsto> tsMap Bool\<cdot> (fst (tsRec\<cdot>(tsMap invBoolPair\<cdot>(ta . dr)))),
                               abpOut \<mapsto> tsMap Data\<cdot> (snd (tsRec\<cdot>(tsMap invBoolPair\<cdot>(ta . dr))))]\<Omega>"
         using recv_mono by blast
       have f4: "\<forall>f n. \<not> chain f \<or> tsbDom\<cdot>(f n::'a MABP TSB) = tsbDom\<cdot>(Lub f)"
         by (meson tsbChain_dom_eq2)
       have f5: "\<And> elem_1 .tsbDom\<cdot> ([ar \<mapsto> tsMap Bool\<cdot> (fst (tsRec\<cdot>(tsMap invBoolPair\<cdot>(Y elem_1 . dr))))
-                          , abpOut \<mapsto> tsMap Data\<cdot> (snd (tsRec\<cdot> (tsMap invBoolPair\<cdot>(Y elem_1 . dr))))]\<Omega>) 
+                          , abpOut \<mapsto> tsMap Data\<cdot> (snd (tsRec\<cdot> (tsMap invBoolPair\<cdot>(Y elem_1 . dr))))]\<Omega>)
                           = {ar, abpOut}"
         by (simp add: recv_tsb_dom)
-      have "\<And> v1_0. tsbDom\<cdot> (Y (v1_0 (\<lambda>n. [ar \<mapsto> tsMap Bool\<cdot> (fst (tsRec\<cdot>(tsMap invBoolPair\<cdot>(Y n . dr)))), 
+      have "\<And> v1_0. tsbDom\<cdot> (Y (v1_0 (\<lambda>n. [ar \<mapsto> tsMap Bool\<cdot> (fst (tsRec\<cdot>(tsMap invBoolPair\<cdot>(Y n . dr)))),
                                            abpOut \<mapsto> tsMap Data\<cdot> (snd (tsRec\<cdot> (tsMap invBoolPair\<cdot>(Y n . dr))))]\<Omega>))) = {dr}"
         using f4 a2 a1 by presburger
-      then have "chain (\<lambda>n. [ar \<mapsto> tsMap Bool\<cdot> (fst (tsRec\<cdot>(tsMap invBoolPair\<cdot>(Y n . dr)))), 
+      then have "chain (\<lambda>n. [ar \<mapsto> tsMap Bool\<cdot> (fst (tsRec\<cdot>(tsMap invBoolPair\<cdot>(Y n . dr)))),
                              abpOut \<mapsto> tsMap Data\<cdot> (snd (tsRec\<cdot>(tsMap invBoolPair\<cdot>(Y n . dr))))]\<Omega>)"
         using f3 a1 by (simp add: po_class.chain_def)
-      then show "tsbDom\<cdot> (\<Squnion>n. [ar \<mapsto> tsMap Bool\<cdot> (fst (tsRec\<cdot>(tsMap invBoolPair\<cdot>(Y n . dr)))), 
+      then show "tsbDom\<cdot> (\<Squnion>n. [ar \<mapsto> tsMap Bool\<cdot> (fst (tsRec\<cdot>(tsMap invBoolPair\<cdot>(Y n . dr)))),
                                abpOut \<mapsto> tsMap Data\<cdot> (snd (tsRec\<cdot>(tsMap invBoolPair\<cdot>(Y n . dr))))]\<Omega>) = {abpOut, ar}"
         using f5 f4 by blast
     qed
-      
-      
-    have f3: "\<And>(Y::nat \<Rightarrow> 'a MABP TSB) c::channel. chain Y \<Longrightarrow> tsbDom\<cdot>(\<Squnion>i::nat. Y i) = {dr} 
-              \<Longrightarrow> c = ar \<or> c = abpOut \<Longrightarrow> c = ar \<longrightarrow> 
-              (tsMap::(bool \<Rightarrow> 'a MABP) \<Rightarrow> bool tstream \<rightarrow> 'a MABP tstream) Bool\<cdot>(fst (tsRec\<cdot>(tsMap invBoolPair\<cdot>(Lub Y  .  dr)))) 
+
+
+    have f3: "\<And>(Y::nat \<Rightarrow> 'a MABP TSB) c::channel. chain Y \<Longrightarrow> tsbDom\<cdot>(\<Squnion>i::nat. Y i) = {dr}
+              \<Longrightarrow> c = ar \<or> c = abpOut \<Longrightarrow> c = ar \<longrightarrow>
+              (tsMap::(bool \<Rightarrow> 'a MABP) \<Rightarrow> bool tstream \<rightarrow> 'a MABP tstream) Bool\<cdot>(fst (tsRec\<cdot>(tsMap invBoolPair\<cdot>(Lub Y  .  dr))))
               \<sqsubseteq> (\<Squnion>i::nat. tsMap Bool\<cdot>(fst (tsRec\<cdot>(tsMap invBoolPair\<cdot>(Y i  .  dr)))))"
      by (simp add: recvCH1_contlub to_recvch1)
-       
-   have f4: "\<And>(Y::nat \<Rightarrow> 'a MABP TSB) c::channel. chain Y \<Longrightarrow> tsbDom\<cdot>(\<Squnion>i::nat. Y i) = {dr} 
-               \<Longrightarrow> c = ar \<or> c = abpOut \<Longrightarrow> c = ar \<longrightarrow>  
-              tsMap Data\<cdot>(snd (tsRec\<cdot>(tsMap invBoolPair\<cdot>(Lub Y  .  dr)))) 
+
+   have f4: "\<And>(Y::nat \<Rightarrow> 'a MABP TSB) c::channel. chain Y \<Longrightarrow> tsbDom\<cdot>(\<Squnion>i::nat. Y i) = {dr}
+               \<Longrightarrow> c = ar \<or> c = abpOut \<Longrightarrow> c = ar \<longrightarrow>
+              tsMap Data\<cdot>(snd (tsRec\<cdot>(tsMap invBoolPair\<cdot>(Lub Y  .  dr))))
                \<sqsubseteq> (\<Squnion>i::nat. tsMap Data\<cdot>(snd (tsRec\<cdot>(tsMap invBoolPair\<cdot>(Y i  .  dr)))))"
     by (simp add: recvCH2_contlub to_recvch2)
-       
+
     show "\<And>Y::nat \<Rightarrow> 'a MABP TSB.
        chain Y \<Longrightarrow>
        tsbDom\<cdot>(\<Squnion>i::nat. Y i) = {dr} \<Longrightarrow>
@@ -272,14 +278,14 @@ lemma recvTSPF_cont [simp]:
       apply (simp add: recvTSPF_tsb_getc tsbdom_rep_eq tsbgetch_rep_eq)
       using f3 f4 by fastforce
   qed
-    
-        
-  subsubsection \<open>tspf_well\<close>        
-    
+
+
+  subsubsection \<open>tspf_well\<close>
+
  (* show that the recvTSPF fulfills the tickcount property *)
 lemma recvTSPF_tick: assumes "tsbDom\<cdot>b = {dr}" and "(#\<surd>tsb b) = n"
-  shows "n \<le> (#\<surd>tsb ([ar \<mapsto> tsMap Bool\<cdot>(fst (tsRec\<cdot>(tsMap invBoolPair\<cdot>(b  .  dr)))), 
-                       abpOut \<mapsto> tsMap Data\<cdot>(snd (tsRec\<cdot>(tsMap invBoolPair\<cdot>(b  .  dr))))]\<Omega>))" 
+  shows "n \<le> (#\<surd>tsb ([ar \<mapsto> tsMap Bool\<cdot>(fst (tsRec\<cdot>(tsMap invBoolPair\<cdot>(b  .  dr)))),
+                       abpOut \<mapsto> tsMap Data\<cdot>(snd (tsRec\<cdot>(tsMap invBoolPair\<cdot>(b  .  dr))))]\<Omega>))"
 proof -
   have "(#\<surd>tsb b) = #\<surd>(b . dr)"
     apply (rule tsbtick_single_ch2)
@@ -296,43 +302,156 @@ proof -
       apply (simp add: tsbgetch_rep_eq)
       using f2 f3 by auto
 qed
-  
-      
+
+
   (* recvTSPF is an actual TSPF *)
-lemma recvTSPF_well: 
-  shows "tspf_well (\<Lambda> x. (tsbDom\<cdot>x = {dr}) \<leadsto> 
-                      [ar \<mapsto> (tsMap::(bool \<Rightarrow> 'a MABP) \<Rightarrow> bool tstream \<rightarrow> 'a MABP tstream) 
+lemma recvTSPF_well:
+  shows "tspf_well (\<Lambda> x. (tsbDom\<cdot>x = {dr}) \<leadsto>
+                      [ar \<mapsto> (tsMap::(bool \<Rightarrow> 'a MABP) \<Rightarrow> bool tstream \<rightarrow> 'a MABP tstream)
                             Bool\<cdot>(fst ((tsRec::('a * bool) tstream \<rightarrow> (bool tstream \<times> 'a tstream))\<cdot>
                             ((tsMap invBoolPair)\<cdot>(x . dr)))),
-                       abpOut \<mapsto> (tsMap::('a \<Rightarrow> 'a MABP) \<Rightarrow> 'a tstream \<rightarrow> 'a MABP tstream) 
-                            Data\<cdot>(snd (tsRec\<cdot>((tsMap invBoolPair)\<cdot>(x . dr))))]\<Omega>)"    
+                       abpOut \<mapsto> (tsMap::('a \<Rightarrow> 'a MABP) \<Rightarrow> 'a tstream \<rightarrow> 'a MABP tstream)
+                            Data\<cdot>(snd (tsRec\<cdot>((tsMap invBoolPair)\<cdot>(x . dr))))]\<Omega>)"
   apply (rule tspf_wellI)
     apply (simp_all add: domIff2 recv_tsb_dom)
     by (simp add: recvTSPF_tick)
+
+
+
+
+  subsection \<open>medium_rs\<close>
+
+(*
+
+definition tsMedRSTSPF :: "bool stream \<Rightarrow> 'a MABP TSPF" where
+"tsMedRSTSPF bst\<equiv> Abs_CTSPF (\<lambda> x. (tsbDom\<cdot>x = {ar})
+                           \<leadsto> [as \<mapsto> (tsMap::(bool \<Rightarrow> 'a MABP) \<Rightarrow> bool tstream \<rightarrow> 'a MABP tstream) Bool\<cdot>(tsMed\<cdot>(tsMap invBool\<cdot>(x . ar))\<cdot>bst)]\<Omega>)"
+
+abbreviation tsMedRSAbb  :: "bool stream \<Rightarrow> 'a MABP TSB \<Rightarrow> 'a MABP TSB option" where
+"tsMedRSAbb bst x \<equiv> ((tsbDom\<cdot>x = {ar})
+                           \<leadsto> [as \<mapsto> (tsMap::(bool \<Rightarrow> 'a MABP) \<Rightarrow> bool tstream \<rightarrow> 'a MABP tstream) Bool\<cdot>(tsMed\<cdot>(tsMap invBool\<cdot>(x . ar))\<cdot>bst)]\<Omega>)"
+
+*)
+subsubsection \<open>defs\<close>
+
+definition medRSH :: "bool stream \<Rightarrow> 'a MABP TSB \<Rightarrow> 'a MABP tstream"  where
+"medRSH bst \<equiv> (\<lambda> x. (tsMap::(bool \<Rightarrow> 'a MABP) \<Rightarrow> bool tstream \<rightarrow> 'a MABP tstream) Bool\<cdot>(tsMed\<cdot>(tsMap invBool\<cdot>(x  .  ar))\<cdot>bst))"
+
+lemma medrsh_cont [simp]: "cont (medRSH bst)"
+  by (simp add: medRSH_def)
+
+lemma medrsh_contlub: assumes "chain Y"
+  shows "(medRSH bst) ((\<Squnion>i. Y i)) = (\<Squnion>i. ((medRSH bst) ((Y i))))"
+  apply (rule cont2contlubE)
+  by (simp_all add: assms)
+
+lemma to_medrsh: "tsMap Bool\<cdot>(tsMed\<cdot>(tsMap invBool\<cdot>(x  .  ar))\<cdot>bst)
+                  = ((medRSH :: bool stream \<Rightarrow> 'a MABP TSB \<Rightarrow> 'a MABP tstream) bst) x"
+  by (simp add: medRSH_def)
+
+subsubsection \<open>pre\<close>
+
+lemma tsmed_input_cont [simp]: "cont (\<lambda> x. tsMed\<cdot>x\<cdot>bst)"
+  by simp
+
+lemma tsmed_input_mono [simp]: "monofun (\<lambda> x. tsMed\<cdot>x\<cdot>bst)"
+  using cont2mono tsmed_input_cont by blast
+
+
+lemma medrs_tsb_well [simp]: "tsb_well  [as \<mapsto> tsMap Bool\<cdot>(tsMed\<cdot>(tsMap invBool\<cdot>(x . ar))\<cdot>bst)]"
+  apply (rule tsb_wellI)
+  by (simp add: tsmap_tsdom_range)
+
+lemma medrs_tsb_dom: "tsbDom\<cdot>([as \<mapsto> tsMap Bool\<cdot>(tsMed\<cdot>(tsMap invBool\<cdot>(x . ar))\<cdot>bst)]\<Omega>) = {as}"
+  by (simp add: tsbdom_rep_eq)
+
+
+subsubsection \<open>cont\<close>
+
+  (* prerequirement for the mono proofs of the tspf *)
+lemma medrs_tsb_mono: "\<And>(x::'a MABP TSB) y::'a MABP TSB.
+       tsbDom\<cdot>x = {ar} \<Longrightarrow> x \<sqsubseteq> y \<Longrightarrow> [as \<mapsto> (tsMap::(bool \<Rightarrow> 'a MABP) \<Rightarrow> bool tstream \<rightarrow> 'a MABP tstream) Bool\<cdot>(tsMed\<cdot>(tsMap invBool\<cdot>(x  .  ar))\<cdot>bst)]\<Omega> \<sqsubseteq> [as \<mapsto> tsMap Bool\<cdot>(tsMed\<cdot>(tsMap invBool\<cdot>(y  .  ar))\<cdot>bst)]\<Omega>"
+  apply (simp_all add: tsbdom_below tsbdom_rep_eq tsbgetch_rep_eq)
+  apply (rule tsb_below)
+    apply (simp_all add: tsbdom_below tsbdom_rep_eq  tsbgetch_rep_eq)
+    apply (simp add: to_medrsh)
+    using cont2mono medrsh_cont monofun_def by blast
+
+
+lemma medrs_mono [simp]: "monofun (\<lambda> x::'a MABP TSB. (tsbDom\<cdot>x = {ar})
+                           \<leadsto> [as \<mapsto> (tsMap::(bool \<Rightarrow> 'a MABP) \<Rightarrow> bool tstream \<rightarrow> 'a MABP tstream)
+                                Bool\<cdot>(tsMed\<cdot>(tsMap invBool\<cdot>(x . ar))\<cdot>bst)]\<Omega>)"
+  apply (rule tspf_monoI)
+  by (simp add: medrs_tsb_mono)
+
+lemma medrs_tsb_getc: assumes "chain (Y::nat \<Rightarrow> 'a MABP TSB)" and "tsbDom\<cdot>(\<Squnion>i::nat. Y i) = {ar}"
+                      and "c = as"
+  shows "(\<Squnion>i::nat. [as \<mapsto> (tsMap::(bool \<Rightarrow> 'a MABP) \<Rightarrow> bool tstream \<rightarrow> 'a MABP tstream) Bool\<cdot>(tsMed\<cdot>(tsMap invBool\<cdot>(Y i  .  ar))\<cdot>bst)]\<Omega>)  .  as
+          =  (\<Squnion>i::nat. ([as \<mapsto> (tsMap::(bool \<Rightarrow> 'a MABP) \<Rightarrow> bool tstream \<rightarrow> 'a MABP tstream) Bool\<cdot>(tsMed\<cdot>(tsMap invBool\<cdot>(Y i  .  ar))\<cdot>bst)]\<Omega>) . as)"
+proof (rule lubgetCh)
+  have f2: "\<And> i. tsbDom\<cdot>(Y i) =  tsbDom\<cdot>(\<Squnion>i. Y i)"
+    by (simp add: assms(1))
+  show tb_chain: "chain (\<lambda>i::nat. [as \<mapsto> (tsMap::(bool \<Rightarrow> 'a MABP) \<Rightarrow> bool tstream \<rightarrow> 'a MABP tstream) Bool\<cdot>(tsMed\<cdot>(tsMap invBool\<cdot>(Y i  .  ar))\<cdot>bst)]\<Omega>)"
+    by (simp add: assms(1) assms(2) po_class.chainE po_class.chainI medrs_tsb_mono)
+  show "as \<in> tsbDom\<cdot>(\<Squnion>i::nat. [as \<mapsto> (tsMap::(bool \<Rightarrow> 'a MABP) \<Rightarrow> bool tstream \<rightarrow> 'a MABP tstream) Bool\<cdot>(tsMed\<cdot>(tsMap invBool\<cdot>(Y i  .  ar))\<cdot>bst)]\<Omega>)"
+    using assms(3) medrs_tsb_dom tb_chain tsbChain_dom_eq2 by blast
+qed
+
+
+
+lemma medrs_cont [simp]: "cont (\<lambda> x::'a MABP TSB. (tsbDom\<cdot>x = {ar})
+                           \<leadsto> [as \<mapsto> (tsMap::(bool \<Rightarrow> 'a MABP) \<Rightarrow> bool tstream \<rightarrow> 'a MABP tstream)
+                                Bool\<cdot>(tsMed\<cdot>(tsMap invBool\<cdot>(x . ar))\<cdot>bst)]\<Omega>)"
+proof (rule tspf_contI)
+  show medrs_mo : "\<And>(x::'a MABP TSB) y::'a MABP TSB. tsbDom\<cdot>x = {ar} \<Longrightarrow> x \<sqsubseteq> y \<Longrightarrow>
+          [as \<mapsto> (tsMap::(bool \<Rightarrow> 'a MABP) \<Rightarrow> bool tstream \<rightarrow> 'a MABP tstream) Bool\<cdot>
+                  (tsMed\<cdot>(tsMap invBool\<cdot>(x  .  ar))\<cdot>bst)]\<Omega>
+          \<sqsubseteq> [as \<mapsto> tsMap Bool\<cdot>(tsMed\<cdot>(tsMap invBool\<cdot>(y  .  ar))\<cdot>bst)]\<Omega>"
+    by (simp add: medrs_tsb_mono)
+
+  have f1: " \<And>Y::nat \<Rightarrow> 'a MABP TSB. chain Y \<Longrightarrow> tsbDom\<cdot>(\<Squnion>i::nat. Y i) = {ar} \<Longrightarrow>
+       tsbDom\<cdot>(\<Squnion>i::nat. [as \<mapsto> (tsMap::(bool \<Rightarrow> 'a MABP) \<Rightarrow> bool tstream \<rightarrow> 'a MABP tstream) Bool\<cdot>(tsMed\<cdot>(tsMap invBool\<cdot>(Y i  .  ar))\<cdot>bst)]\<Omega>) = {as}"
+    by (metis (mono_tags, lifting) medrs_mo medrs_tsb_dom po_class.chainE po_class.chainI tsbChain_dom_eq2)
+
+
+  show "\<And>Y::nat \<Rightarrow> 'a MABP TSB. chain Y \<Longrightarrow> tsbDom\<cdot>(\<Squnion>i::nat. Y i) = {ar} \<Longrightarrow>
+       [as \<mapsto> (tsMap::(bool \<Rightarrow> 'a MABP) \<Rightarrow> bool tstream \<rightarrow> 'a MABP tstream) Bool\<cdot>(tsMed\<cdot>(tsMap invBool\<cdot>((\<Squnion>i::nat. Y i)  .  ar))\<cdot>bst)]\<Omega> \<sqsubseteq> (\<Squnion>i::nat. [as \<mapsto> tsMap Bool\<cdot>(tsMed\<cdot>(tsMap invBool\<cdot>(Y i  .  ar))\<cdot>bst)]\<Omega>)"
+    apply (rule tsb_below)
+      apply (simp_all add: tsbdom_below tsbdom_rep_eq tsbgetch_rep_eq f1)
+      apply (simp add: medrs_tsb_getc tsbdom_rep_eq tsbgetch_rep_eq)
+       by (simp add: medrsh_contlub to_medrsh)
+qed
+
+
+  subsubsection \<open>tspf_well\<close>
+  
+ (* show that the mediumRSTSPF template  fulfills the tickcount property *)
+lemma medrs_tick: assumes "tsbDom\<cdot>b = {ar}" and "(#\<surd>tsb b) = n" and "#bst=\<infinity>"
+  shows "n \<le> (#\<surd>tsb [as \<mapsto> (tsMap::(bool \<Rightarrow> 'a MABP) \<Rightarrow> bool tstream \<rightarrow> 'a MABP tstream) Bool\<cdot>(tsMed\<cdot>(tsMap invBool\<cdot>(b  .  ar))\<cdot>bst)]\<Omega>)"
+proof -
+  have "(#\<surd>tsb b) = #\<surd>(b . ar)"
+    apply (rule tsbtick_single_ch2)
+    by (simp add: assms(1))
+  hence f1: "n = #\<surd>(b . ar)"
+    using assms(2) by blast
+  hence f2: "n \<le> #\<surd>((tsMap::(bool \<Rightarrow> 'a MABP) \<Rightarrow> bool tstream \<rightarrow> 'a MABP tstream) Bool\<cdot>(tsMed\<cdot>(tsMap invBool\<cdot>(b  .  ar))\<cdot>bst))"
+    by (simp add: assms(3))
+  show ?thesis
+    apply (rule tsbtick_geI)
+    apply (simp add: medrs_tsb_dom tsbgetch_rep_eq)
+    using f2 by force
+qed
+  
+      
     
-    
-    
-    
-    
-    
-    
-    
-    
-    
-    
-    
-    
-    
-    
-    
-    
-    
-    
-    
-    
-    
-    
-    
-    
+  (* a medium is a tspf if the oracle bool stream bst is infinitly long*)
+lemma medrs_well: assumes "#bst=\<infinity>"
+shows "tspf_well (\<Lambda> x. (tsbDom\<cdot>x = {ar})
+                           \<leadsto> [as \<mapsto> (tsMap::(bool \<Rightarrow> 'a MABP) \<Rightarrow> bool tstream \<rightarrow> 'a MABP tstream)
+                                Bool\<cdot>(tsMed\<cdot>(tsMap invBool\<cdot>(x . ar))\<cdot>bst)]\<Omega>)"
+  apply (rule tspf_wellI)
+    apply (simp_all add: domIff2 medrs_tsb_dom)
+    apply (subst tsbtick_single_ch1, simp)
+    by (simp add: assms tsbtick_single_ch2)
     
 end
